\begin{formula}
a^2+b^2=c^2
\end{formula}
\begin{formula}
\int_\Omega \phi \mathrm{d} \mu = \sum_{i=1}^{n} \alpha_i \mu(A_i)
\end{formula}
\begin{formula}
\int_{-\infty}^{\infty} e^{-x^2}\mathrm{d}x=\sqrt{\pi}
\end{formula}
\begin{formula}
(6 \cdot 9) + (6+9) = 69
\end{formula}
\begin{formula}
\int_a^b f(x)\mathrm{d}x = F(b) - F(a)
\end{formula}
\begin{formula}
\frac{1}{\sqrt{2\pi}\sigma}e^{-\frac{(x-\mu)^2}{2 \sigma^2}}
\end{formula}
\begin{formula}
e^{i\pi}+1=0
\end{formula}
\begin{formula}
\sum_{k=0}^\infty q^k=\frac{1}{1-q}
\end{formula}
\begin{formula}
\frac{1}{\pi} = \frac{2 \sqrt 2}{99^2} \sum_{k=0}^\infty \frac{(4k)!}{k!^4} \frac{26390k+1103}{396^{4k}}
\end{formula}
\begin{formula}
\Gamma(z) = \int_0^\infty t^{z-1} e^{-t} \mathrm dt
\end{formula}
\begin{formula}
f_n = f_{n-1} + f_{n-2}
\end{formula}
\begin{formula}
f_n = f_{n-1} + f_{n-2}
\end{formula}
\begin{formula}
\frac {{1}}{{2}} < \left\lfloor \bmod \left({{\left\lfloor \frac {{y}}{{17}}\right\rfloor 2^{{-17\lfloor x\rfloor -\bmod ({{\lfloor y\rfloor }}, {{17}})}}}}, 2\right)\right\rfloor
\end{formula}
\begin{formula}
\| x \|_p = \left(\sum_{i=1}^n | x_i |^p\right)^{1/p}
\end{formula}
\begin{formula}
0!=1
\end{formula}
\begin{formula}
\sin^2 \alpha+\cos^2 \alpha = 1
\end{formula}
\begin{formula}
\zeta(s) =\sum_{n=1}^\infty\frac{1}{n^s}
\end{formula}
\begin{formula}
\frac{1}{\sqrt{2}+1}=\sqrt{2}-1
\end{formula}
\begin{formula}
0.999... = 1
\end{formula}
\begin{formula}
\sum_{k=1}^\infty \frac{1}{k^2}=\frac{\pi^2}{6}
\end{formula}
\begin{formula}
\int u \, v'=uv-\int v \, u'
\end{formula}
\begin{formula}
\sum_{k=1}^nk=\frac{n(n+1)}{2}
\end{formula}
\begin{formula}
|a+b| \le |a| + |b|
\end{formula}
\begin{formula}
(1+x)^n \geq 1+nx
\end{formula}
\begin{formula}
(x+y)^n = \sum_{k=0}^{n}\binom{n}{k} x^{n-k}y^{k}
\end{formula}
\begin{formula}
\binom nk = \frac{n!}{k! \cdot (n-k)!}
\end{formula}
\begin{formula}
(f^{-1})'(y) = \frac{1}{f'(f^{-1}(y))} = \frac{1}{f'(x)}
\end{formula}
\begin{formula}
\lim_{n\to\infty} \left(1+\frac {z}{n}\right)^n=e^z
\end{formula}
\begin{formula}
\lim_{n\to\infty}\left(1+\frac12+\frac13+\dotsb+\frac1{n}-\ln n\right) = \gamma
\end{formula}
\begin{formula}
\forall \varepsilon>0 \; \exists N\in\mathbb{N} \; \forall n>N: \;\left|a_n-a \right|<\varepsilon
\end{formula}
\begin{formula}
e
=
\frac{2}{1}
\sqrt[2]{\frac{4}{3}}
\sqrt[4]{\frac{6}{5}\frac{8}{7}}
\sqrt[8]{\frac{10}{9}\frac{12}{11}\frac{14}{13}\frac{16}{15}}
...
\end{formula}
\begin{formula}
\lim_{x \to p} \frac{f(x) - f(p)- L(x-p)}{\|x-p\|} = 0
\end{formula}
\begin{formula}
\operatorname{P}\left[\left|X-\mu\right|\geq k\right] \leq \frac{\sigma^2}{k^2}
\end{formula}
\begin{formula}
e^{ix} = \cos x + i\sin x
\end{formula}
\begin{formula}
\exp(x) = \sum_{n = 0}^\infty \frac{x^n}{n!}
\end{formula}
\begin{formula}
\|fg\|_1 \le \|f\|_p \|g\|_q
\end{formula}
\begin{formula}
P(A\mid B) = \frac{P(B \mid A) \, P(A)}{P(B)}
\end{formula}
\begin{formula}
    \left( \sum_{k=1}^n a_k b_k \right)^2 \leq
    \left( \sum_{k=1}^n a_k^2 \right)
    \left( \sum_{k=1}^n b_k^2 \right)
\end{formula}
\begin{formula}
{\cosh}^2 (z) - {\sinh}^2 (z) = 1
\end{formula}
\begin{formula}
P_\lambda (k) = \frac{\lambda^k}{k!}\, \mathrm{e}^{-\lambda}
\end{formula}
\begin{formula}
\sin(x) = x \prod_{k=1}^\infty \left( 1 - \frac{x^2}{k^2\pi^2} \right)
\end{formula}
\begin{formula}
\cos(x) = \prod_{k=1}^\infty \left( 1 - \frac{4x^2}{(2k-1)^2\pi^2} \right)
\end{formula}
\begin{formula}
\cosh x + \sinh x = e^x
\end{formula}
\begin{formula}
f(x) = f(-x)
\end{formula}
\begin{formula}
-f(x) = f(-x)
\end{formula}
\begin{formula}
f(x+p) = f(x)
\end{formula}
\begin{formula}
n! \sim \sqrt{2 \pi n}\left(\frac{n}{e}\right)^n
\end{formula}
\begin{formula}
\Gamma\left({\frac{1}{2}}\right)=\sqrt{\pi}
\end{formula}
\begin{formula}
e=\lim_{n \to \infty} \frac{n}{\sqrt[n]{n!}}
\end{formula}
\begin{formula}
x_{1,2} = - \frac{p}{2}\pm\sqrt{\left(\frac{p}2\right)^2 - q}
\end{formula}
\begin{formula}
x_{1,2} = \frac{-b\pm\sqrt{b^2-4ac}}{2a}
\end{formula}
\begin{formula}
\forall \varepsilon > 0\; \exists \delta > 0\; \forall x:\;| x - p | < \delta \Rightarrow | f(x) - f(p) | < \varepsilon
\end{formula}
\begin{formula}
\sum_{n=0} ^ {\infty} \frac {f^{(n)}(a)}{n!} \, (x-a)^{n}
\end{formula}
\begin{formula}
F(s) = \int_0^\infty f(t)e^{-st} \, dt
\end{formula}
\begin{formula}
\hat{f}(\xi) = \int_{-\infty}^{\infty} f(x)\ e^{-2\pi i x \xi}\,dx
\end{formula}
\begin{formula}
\frac 1 \pi=12 \sum^\infty_{k=0} \frac{(-1)^k (6k)! (13591409 + 545140134k)}{(3k)!(k!)^3 640320^{3k + 3/2}}
\end{formula}
\begin{formula}
\frac{1}{1 + x^2} = \frac12 \left( \frac{1}{1- ix} + \frac{1}{1 + ix}\right) % bernoulli
\end{formula}
\begin{formula}
\pi = \frac{\sqrt{3}}{6^5} \sum_{k = 0}^{\infty} \frac{((4k)!)^2(6k)!}{9^{k+1}(12k)!(2k)!} \left( \frac{127169}{12k + 1} - \frac{1070}{12k + 5} - \frac{131}{12k + 7} + \frac{2}{12k + 11}\right)
\end{formula}
\begin{formula}
\sum_{k=0}^n\binom{n}{k}=2^n
\end{formula}
\begin{formula}
\binom{n}{k}=\binom{n-1}{k-1}+\binom{n-1}{k}
\end{formula}
\begin{formula}
\int_0^1 x^{-x}\,dx = \sum_{n=1}^\infty n^{-n} % sophomores dream
\end{formula}
\begin{formula}
\Gamma(z) \, \Gamma (1-z)=\frac{\pi}{\sin(\pi z)} \qquad z\in\mathbb{C}\setminus\mathbb{Z} % Eulerscher Ergaenzungssatz
\end{formula}
\begin{formula}
\Gamma'(1)=-\gamma
\end{formula}
\begin{formula}
\frac{\Gamma\left(\frac{1}{24}\right) \,\Gamma\left(\frac{11}{24}\right)}{\Gamma\left(\frac{5}{24}\right) \, \Gamma\left(\frac{7}{24}\right)}=\sqrt{3}\cdot\sqrt{2+\sqrt{3}}
\end{formula}
\begin{formula}
\zeta(z)=2\, (2\pi)^{z-1}\, \zeta(1-z)\, \Gamma(1-z)\, \sin\frac{\pi z}{2} % riemannsche funktionalgleichung
\end{formula}
\begin{formula}
\sum_{k=0}^n \frac{1}{{\binom{n}{k}}}=\frac{n+1}{2^{n+1}} \sum_{k=1}^{n+1} \frac{2^k}{k}
\end{formula}
\begin{formula}
\frac{1}{\pi}\int_0^\pi \dfrac{\sin^{z}(t)}{\sin^{k}(\frac{k}{z}t)\sin^{z-k}(\frac{z-k}{z}t)}\,dt = \dbinom{z}{k}
\end{formula}
\begin{formula}
r = \frac{1}{\limsup_{n\rightarrow\infty}\sqrt[n]{|z_n|}}
\end{formula}
\begin{formula}
r = \lim_{n\rightarrow\infty} \left| \frac{z_{n}}{z_{n+1}} \right|
\end{formula}